feat: `simp +arith` normalizes coefficient in linear integer polynomials (#7015)
This PR makes sure `simp +arith` normalizes coefficients in linear
integer polynomials. There is still one todo: tightening the bound of
inequalities.

src/Init/Data/Int/Linear.lean
@@ -8,6 +8,7 @@ import Init.ByCases
 import Init.Data.Prod
 import Init.Data.Int.Lemmas
 import Init.Data.Int.LemmasAux
+import Init.Data.Int.DivModLemmas
 import Init.Data.RArray
 
 namespace Int.Linear
@@ -97,9 +98,33 @@ def PolyCnstr.denote (ctx : Context) : PolyCnstr → Prop
   | .eq p => p.denote ctx = 0
   | .le p => p.denote ctx ≤ 0
 
+def Poly.div (k : Int) : Poly → Poly
+  | .num k' => .num (k'/k)
+  | .add k' x p => .add (k'/k) x (div k p)
+
+def Poly.divAll (k : Int) : Poly → Bool
+  | .num k' => (k'/k)*k == k'
+  | .add k' _ p => (k'/k)*k == k' && divAll k p
+
+def Poly.divCoeffs (k : Int) : Poly → Bool
+  | .num _ => true
+  | .add k' _ p => (k'/k)*k == k' && divCoeffs k p
+
+def Poly.getConst : Poly → Int
+  | .num k => k
+  | .add _ _ p => getConst p
+
 def PolyCnstr.norm : PolyCnstr → PolyCnstr
   | .eq p => .eq p.norm
   | .le p => .le p.norm
+
+def PolyCnstr.divAll (k : Int) : PolyCnstr → Bool
+  | .eq p => p.divAll k
+  | .le p => p.divAll k
+
+def PolyCnstr.div (k : Int) : PolyCnstr → PolyCnstr
+  | .eq p => .eq <| p.div k
+  | .le p => .le <| p.div k
 
 inductive ExprCnstr  where
   | eq (p₁ p₂ : Expr)
@@ -113,6 +138,10 @@ def ExprCnstr.denote (ctx : Context) : ExprCnstr → Prop
 def ExprCnstr.toPoly : ExprCnstr → PolyCnstr
   | .eq e₁ e₂ => .eq (e₁.sub e₂).toPoly.norm
   | .le e₁ e₂ => .le (e₁.sub e₂).toPoly.norm
+
+-- Certificate for normalizing the coefficients of a constraint
+def divBy (e e' : ExprCnstr) (k : Int) : Bool :=
+  k > 0 && e.toPoly.divAll k && e'.toPoly == e.toPoly.div k
 
 attribute [local simp] Int.add_comm Int.add_assoc Int.add_left_comm Int.add_mul Int.mul_add
 attribute [local simp] Poly.insert Poly.denote Poly.norm Poly.addConst
@@ -143,7 +172,30 @@ private theorem sub_fold (a b : Int) : a.sub b = a - b := rfl
 private theorem neg_fold (a : Int) : a.neg = -a := rfl
 
 attribute [local simp] sub_fold neg_fold
-attribute [local simp] ExprCnstr.denote ExprCnstr.toPoly PolyCnstr.denote Expr.denote
+
+attribute [local simp] Poly.div Poly.divAll PolyCnstr.denote
+
+theorem Poly.denote_div_eq_of_divAll (ctx : Context) (p : Poly) (k : Int) : p.divAll k → (p.div k).denote ctx * k = p.denote ctx := by
+  induction p with
+  | num _ => simp
+  | add k' v p ih =>
+    simp; intro h₁ h₂
+    have ih := ih h₂
+    simp [ih]
+    apply congrArg (denote ctx p + ·)
+    rw [Int.mul_right_comm, h₁]
+
+attribute [local simp] Poly.divCoeffs Poly.getConst
+
+theorem Poly.denote_div_eq_of_divCoeffs (ctx : Context) (p : Poly) (k : Int) : p.divCoeffs k → (p.div k).denote ctx * k + p.getConst % k = p.denote ctx := by
+  induction p with
+  | num k' => simp; rw [Int.add_comm, Int.mul_comm, Int.ediv_add_emod]
+  | add k' v p ih =>
+    simp; intro h₁ h₂
+    rw [← ih h₂]
+    rw [Int.mul_right_comm, h₁, Int.add_assoc]
+
+attribute [local simp] ExprCnstr.denote ExprCnstr.toPoly Expr.denote
 
 theorem Expr.denote_toPoly'_go (ctx : Context) (e : Expr) :
   (toPoly'.go k e p).denote ctx = k * e.denote ctx + p.denote ctx := by
@@ -172,7 +224,7 @@ theorem Expr.denote_toPoly'_go (ctx : Context) (e : Expr) :
 theorem Expr.denote_toPoly (ctx : Context) (e : Expr) : e.toPoly.denote ctx = e.denote ctx := by
   simp [toPoly, toPoly', Expr.denote_toPoly'_go]
 
-attribute [local simp] Expr.denote_toPoly
+attribute [local simp] Expr.denote_toPoly PolyCnstr.denote
 
 theorem ExprCnstr.denote_toPoly (ctx : Context) (c : ExprCnstr) : c.toPoly.denote ctx = c.denote ctx := by
   cases c <;> simp
@@ -228,6 +280,61 @@ theorem ExprCnstr.eq_of_toPoly_eq_const (ctx : Context) (x : Var) (k : Int) (c :
   rw [h]; simp
   rw [Int.add_comm, ← Int.sub_eq_add_neg, Int.sub_eq_zero]
 
+private theorem mul_eq_zero_iff_eq_zero (a b : Int) : b ≠ 0 → (a * b = 0 ↔ a = 0) := by
+  intro h
+  constructor
+  · intro h'
+    cases Int.mul_eq_zero.mp h'
+    · assumption
+    · contradiction
+  · intro; simp [*]
+
+private theorem eq_mul_le_zero {a b : Int} : 0 < b → (a ≤ 0 ↔ a * b ≤ 0) := by
+  intro h
+  have : 0 = 0 * b := by simp
+  constructor
+  · intro h'
+    rw [this]
+    apply Int.mul_le_mul h' <;> try simp
+    apply Int.le_of_lt h
+  · intro h'
+    rw [this] at h'
+    exact Int.le_of_mul_le_mul_right h' h
+
+attribute [local simp] PolyCnstr.divAll PolyCnstr.div
+
+theorem ExprCnstr.eq_of_toPoly_eq_of_divBy' (ctx : Context) (e e' : ExprCnstr) (p : PolyCnstr) (k : Int) : k > 0 → p.divAll k → e.toPoly = p → e'.toPoly = p.div k → e.denote ctx = e'.denote ctx := by
+  intro h₀ h₁ h₂ h₃
+  have hz : k ≠ 0 := by intro h; simp [h] at h₀
+  cases p <;> simp at h₁
+  next p =>
+    replace h₁ := Poly.denote_div_eq_of_divAll ctx p k h₁
+    replace h₂ := congrArg (PolyCnstr.denote ctx) h₂
+    simp only [PolyCnstr.denote.eq_1, ← h₁] at h₂
+    replace h₃ := congrArg (PolyCnstr.denote ctx) h₃
+    simp only [PolyCnstr.denote.eq_1, PolyCnstr.div] at h₃
+    rw [mul_eq_zero_iff_eq_zero _ _ hz] at h₂
+    have := Eq.trans h₂ h₃.symm
+    rw [denote_toPoly, denote_toPoly] at this
+    exact this
+  next p =>
+    -- TODO: this is correct but we can simplify `p ≤ 0` if `p.divCoeffs k` and `p.getConst % k > 0`. Here, we are simplifying only the case `p.getConst % k = 0`
+    replace h₁ := Poly.denote_div_eq_of_divAll ctx p k h₁
+    replace h₂ := congrArg (PolyCnstr.denote ctx) h₂
+    simp only [PolyCnstr.denote.eq_2, ← h₁] at h₂
+    replace h₃ := congrArg (PolyCnstr.denote ctx) h₃
+    simp only [PolyCnstr.denote.eq_2, PolyCnstr.div] at h₃
+    rw [eq_mul_le_zero h₀] at h₃
+    have := Eq.trans h₂ h₃.symm
+    rw [denote_toPoly, denote_toPoly] at this
+    exact this
+
+theorem ExprCnstr.eq_of_toPoly_eq_of_divBy (ctx : Context) (e e' : ExprCnstr) (k : Int) : divBy e e' k → e.denote ctx = e'.denote ctx := by
+  intro h
+  simp only [divBy, Bool.and_eq_true, bne_iff_ne, ne_eq, beq_iff_eq, decide_eq_true_eq] at h
+  have ⟨⟨h₁, h₂⟩, h₃⟩ := h
+  exact ExprCnstr.eq_of_toPoly_eq_of_divBy' ctx e e' e.toPoly k h₁ h₂ rfl h₃
+
 def PolyCnstr.isUnsat : PolyCnstr → Bool
   | .eq (.num k) => k != 0
   | .eq _ => false
@@ -242,6 +349,43 @@ theorem ExprCnstr.eq_false_of_isUnsat (ctx : Context) (c : ExprCnstr) (h : c.toP
   have := PolyCnstr.eq_false_of_isUnsat ctx (c.toPoly) h
   rw [ExprCnstr.denote_toPoly] at this
   assumption
+
+def PolyCnstr.isUnsatCoeff (k : Int) : PolyCnstr → Bool
+  | .eq p => p.divCoeffs k && k > 0 && p.getConst % k > 0
+  | .le _ => false
+
+private theorem contra {a b k : Int} (h₀ : 0 < k) (h₁ : 0 < b) (h₂ : b < k) (h₃ : a*k + b = 0) : False := by
+  have : b = -a*k := by
+    rw [← Int.neg_eq_of_add_eq_zero h₃, Int.neg_mul]
+  rw [this] at h₁ h₂
+  conv at h₂ => rhs; rw [← Int.one_mul k]
+  have high := Int.lt_of_mul_lt_mul_right h₂ (Int.le_of_lt h₀)
+  rw [← Int.zero_mul k] at h₁
+  have low := Int.lt_of_mul_lt_mul_right h₁ (Int.le_of_lt h₀)
+  replace low : 1 ≤ -a := low
+  have : (1 : Int) < 1 := Int.lt_of_le_of_lt low high
+  contradiction
+
+private theorem PolyCnstr.eq_false (ctx : Context) (p : Poly) (k : Int) : p.divCoeffs k → k > 0 → p.getConst % k > 0 → (PolyCnstr.eq p).denote ctx = False := by
+  simp
+  intro h₁ h₂ h₃ h
+  have hnz : k ≠ 0 := by intro h; rw [h] at h₂; contradiction
+  have := Poly.denote_div_eq_of_divCoeffs ctx p k h₁
+  rw [h] at this
+  have low := h₃
+  have high := Int.emod_lt_of_pos p.getConst h₂
+  exact contra h₂ low high this
+
+theorem ExprCnstr.eq_false_of_isUnsat_coeff (ctx : Context) (c : ExprCnstr) (k : Int) : c.toPoly.isUnsatCoeff k → c.denote ctx = False := by
+  intro h
+  cases c <;> simp [toPoly, PolyCnstr.isUnsatCoeff] at h
+  next e₁ e₂ =>
+    have ⟨⟨h₁, h₂⟩, h₃⟩ := h
+    have := PolyCnstr.eq_false ctx _ _ h₁ h₂ h₃
+    simp at this
+    simp
+    intro he
+    simp [he] at this
 
 def PolyCnstr.isValid : PolyCnstr → Bool
   | .eq (.num k) => k == 0
